Update cdc6600_scoreboard.v

cdc6600_scoreboard.v
@@ -36,6 +36,32 @@ Inductive func_unit : Type :=
   | FU_Incr1
   | FU_Incr2.
 
+(** Functional unit equality *)
+Definition func_unit_eq (fu1 fu2 : func_unit) : bool :=
+  match fu1, fu2 with
+  | FU_Branch, FU_Branch | FU_Boolean, FU_Boolean | FU_Shift, FU_Shift
+  | FU_LongAdd, FU_LongAdd | FU_FPAdd, FU_FPAdd | FU_FPMul1, FU_FPMul1
+  | FU_FPMul2, FU_FPMul2 | FU_FPDiv, FU_FPDiv | FU_Incr1, FU_Incr1 | FU_Incr2, FU_Incr2 => true
+  | _, _ => false
+  end.
+
+(** Functional unit equality correctness *)
+Lemma func_unit_eq_spec : forall fu1 fu2, func_unit_eq fu1 fu2 = true <-> fu1 = fu2.
+Proof.
+  intros fu1 fu2. split.
+  - intro H. destruct fu1, fu2; try reflexivity; discriminate H.
+  - intro H. rewrite H. destruct fu2; reflexivity.
+Qed.
+
+(** Functional unit decidable equality *)
+Lemma func_unit_eq_dec : forall fu1 fu2 : func_unit, {fu1 = fu2} + {fu1 <> fu2}.
+Proof.
+  intros fu1 fu2.
+  destruct (func_unit_eq fu1 fu2) eqn:Heq.
+  - left. apply func_unit_eq_spec. assumption.
+  - right. intro Hcontra. apply func_unit_eq_spec in Hcontra. rewrite Hcontra in Heq. discriminate.
+Qed.
+
 (** Q-numbers encode result provenance:
     - QFU fu: Result pending from functional unit fu
     - QNone: No result pending
@@ -874,6 +900,79 @@ Definition fu_for_op (op : operation) (fus : fu_status) : func_unit :=
   | Op_Incr _ => if fu_busy (fus FU_Incr1) then FU_Incr2 else FU_Incr1
   end.
 
+(** fu_for_op always returns a valid functional unit *)
+Lemma fu_for_op_valid : forall op fus,
+  match fu_for_op op fus with
+  | FU_Branch | FU_Boolean | FU_Shift | FU_LongAdd | FU_FPAdd
+  | FU_FPMul1 | FU_FPMul2 | FU_FPDiv | FU_Incr1 | FU_Incr2 => True
+  end.
+Proof.
+  intros op fus.
+  destruct op; simpl; auto.
+  - destruct (fu_busy (fus FU_FPMul1)); auto.
+  - destruct (fu_busy (fus FU_Incr1)); auto.
+Qed.
+
+(** FU allocation for multiply operations *)
+Lemma fu_for_fpmul_cases : forall fus,
+  fu_for_op (Op_FPMul OP_FMUL) fus = FU_FPMul1 \/
+  fu_for_op (Op_FPMul OP_FMUL) fus = FU_FPMul2.
+Proof.
+  intro fus. simpl.
+  destruct (fu_busy (fus FU_FPMul1)); [right|left]; reflexivity.
+Qed.
+
+(** FU allocation for increment operations *)
+Lemma fu_for_incr_cases : forall iop fus,
+  fu_for_op (Op_Incr iop) fus = FU_Incr1 \/
+  fu_for_op (Op_Incr iop) fus = FU_Incr2.
+Proof.
+  intros iop fus. simpl.
+  destruct (fu_busy (fus FU_Incr1)); [right|left]; reflexivity.
+Qed.
+
+(** Unique FU for branch operations *)
+Lemma fu_for_branch_unique : forall bop fus,
+  fu_for_op (Op_Branch bop) fus = FU_Branch.
+Proof.
+  intros. reflexivity.
+Qed.
+
+(** Unique FU for boolean operations *)
+Lemma fu_for_bool_unique : forall bop fus,
+  fu_for_op (Op_Bool bop) fus = FU_Boolean.
+Proof.
+  intros. reflexivity.
+Qed.
+
+(** Unique FU for shift operations *)
+Lemma fu_for_shift_unique : forall sop fus,
+  fu_for_op (Op_Shift sop) fus = FU_Shift.
+Proof.
+  intros. reflexivity.
+Qed.
+
+(** Unique FU for long add operations *)
+Lemma fu_for_longadd_unique : forall lop fus,
+  fu_for_op (Op_LongAdd lop) fus = FU_LongAdd.
+Proof.
+  intros. reflexivity.
+Qed.
+
+(** Unique FU for FP add operations *)
+Lemma fu_for_fpadd_unique : forall fop fus,
+  fu_for_op (Op_FPAdd fop) fus = FU_FPAdd.
+Proof.
+  intros. reflexivity.
+Qed.
+
+(** Unique FU for FP divide operations *)
+Lemma fu_for_fpdiv_unique : forall dop fus,
+  fu_for_op (Op_FPDiv dop) fus = FU_FPDiv.
+Proof.
+  intros. reflexivity.
+Qed.
+
 (** Structural hazard: required functional unit is busy *)
 Definition structural_hazard (fus : fu_status) (instr : instruction) : Prop :=
   fu_busy (fus (fu_for_op (instr_op instr) fus)) = true.
@@ -885,23 +984,109 @@ Proof.
   intros. unfold structural_hazard. tauto.
 Qed.
 
+(** X register equality *)
+Definition xreg_eq (x1 x2 : xreg) : bool :=
+  match x1, x2 with
+  | X0, X0 | X1, X1 | X2, X2 | X3, X3 | X4, X4 | X5, X5 | X6, X6 | X7, X7 => true
+  | _, _ => false
+  end.
+
+(** X register equality correctness *)
+Lemma xreg_eq_spec : forall x1 x2, xreg_eq x1 x2 = true <-> x1 = x2.
+Proof.
+  intros x1 x2. split.
+  - intro H. destruct x1, x2; try reflexivity; discriminate H.
+  - intro H. rewrite H. destruct x2; reflexivity.
+Qed.
+
+(** X register decidable equality *)
+Lemma xreg_eq_dec : forall x1 x2 : xreg, {x1 = x2} + {x1 <> x2}.
+Proof.
+  intros x1 x2.
+  destruct (xreg_eq x1 x2) eqn:Heq.
+  - left. apply xreg_eq_spec. assumption.
+  - right. intro Hcontra. apply xreg_eq_spec in Hcontra. rewrite Hcontra in Heq. discriminate.
+Qed.
+
+(** A register equality *)
+Definition areg_eq (a1 a2 : areg) : bool :=
+  match a1, a2 with
+  | A0, A0 | A1, A1 | A2, A2 | A3, A3 | A4, A4 | A5, A5 | A6, A6 | A7, A7 => true
+  | _, _ => false
+  end.
+
+(** A register equality correctness *)
+Lemma areg_eq_spec : forall a1 a2, areg_eq a1 a2 = true <-> a1 = a2.
+Proof.
+  intros a1 a2. split.
+  - intro H. destruct a1, a2; try reflexivity; discriminate H.
+  - intro H. rewrite H. destruct a2; reflexivity.
+Qed.
+
+(** A register decidable equality *)
+Lemma areg_eq_dec : forall a1 a2 : areg, {a1 = a2} + {a1 <> a2}.
+Proof.
+  intros a1 a2.
+  destruct (areg_eq a1 a2) eqn:Heq.
+  - left. apply areg_eq_spec. assumption.
+  - right. intro Hcontra. apply areg_eq_spec in Hcontra. rewrite Hcontra in Heq. discriminate.
+Qed.
+
+(** B register equality *)
+Definition breg_eq (b1 b2 : breg) : bool :=
+  match b1, b2 with
+  | B0, B0 | B1, B1 | B2, B2 | B3, B3 | B4, B4 | B5, B5 | B6, B6 | B7, B7 => true
+  | _, _ => false
+  end.
+
+(** B register equality correctness *)
+Lemma breg_eq_spec : forall b1 b2, breg_eq b1 b2 = true <-> b1 = b2.
+Proof.
+  intros b1 b2. split.
+  - intro H. destruct b1, b2; try reflexivity; discriminate H.
+  - intro H. rewrite H. destruct b2; reflexivity.
+Qed.
+
+(** B register decidable equality *)
+Lemma breg_eq_dec : forall b1 b2 : breg, {b1 = b2} + {b1 <> b2}.
+Proof.
+  intros b1 b2.
+  destruct (breg_eq b1 b2) eqn:Heq.
+  - left. apply breg_eq_spec. assumption.
+  - right. intro Hcontra. apply breg_eq_spec in Hcontra. rewrite Hcontra in Heq. discriminate.
+Qed.
+
 (** Register equality *)
 Definition reg_eq (r1 r2 : reg_id) : bool :=
   match r1, r2 with
-  | Reg_X x1, Reg_X x2 => match x1, x2 with
-    | X0, X0 | X1, X1 | X2, X2 | X3, X3 | X4, X4 | X5, X5 | X6, X6 | X7, X7 => true
-    | _, _ => false
-    end
-  | Reg_A a1, Reg_A a2 => match a1, a2 with
-    | A0, A0 | A1, A1 | A2, A2 | A3, A3 | A4, A4 | A5, A5 | A6, A6 | A7, A7 => true
-    | _, _ => false
-    end
-  | Reg_B b1, Reg_B b2 => match b1, b2 with
-    | B0, B0 | B1, B1 | B2, B2 | B3, B3 | B4, B4 | B5, B5 | B6, B6 | B7, B7 => true
-    | _, _ => false
-    end
+  | Reg_X x1, Reg_X x2 => xreg_eq x1 x2
+  | Reg_A a1, Reg_A a2 => areg_eq a1 a2
+  | Reg_B b1, Reg_B b2 => breg_eq b1 b2
   | _, _ => false
   end.
+
+(** Register equality correctness *)
+Lemma reg_eq_spec : forall r1 r2, reg_eq r1 r2 = true <-> r1 = r2.
+Proof.
+  intros r1 r2. split.
+  - intro H. destruct r1, r2; try discriminate H.
+    + apply xreg_eq_spec in H. rewrite H. reflexivity.
+    + apply areg_eq_spec in H. rewrite H. reflexivity.
+    + apply breg_eq_spec in H. rewrite H. reflexivity.
+  - intro H. rewrite H. destruct r2; simpl.
+    + apply xreg_eq_spec. reflexivity.
+    + apply areg_eq_spec. reflexivity.
+    + apply breg_eq_spec. reflexivity.
+Qed.
+
+(** Register decidable equality *)
+Lemma reg_eq_dec : forall r1 r2 : reg_id, {r1 = r2} + {r1 <> r2}.
+Proof.
+  intros r1 r2.
+  destruct (reg_eq r1 r2) eqn:Heq.
+  - left. apply reg_eq_spec. assumption.
+  - right. intro Hcontra. apply reg_eq_spec in Hcontra. rewrite Hcontra in Heq. discriminate.
+Qed.
 
 (** Check if any busy FU will write to a register *)
 Definition reg_reserved (fus : fu_status) (r : reg_id) : bool :=
@@ -1147,6 +1332,30 @@ Definition read_precond (fu : func_unit) (st : scoreboard_state) : Prop :=
   fu_busy (sb_fu_status st fu) = true /\
   ~second_order_conflict (sb_fu_status st fu).
 
+(** Boolean version of read_precond *)
+Definition read_precond_b (fu : func_unit) (st : scoreboard_state) : bool :=
+  andb (fu_busy (sb_fu_status st fu)) (negb (raw_hazard_b (sb_fu_status st fu))).
+
+(** read_precond decidability *)
+Lemma read_precond_dec : forall fu st, {read_precond fu st} + {~read_precond fu st}.
+Proof.
+  intros fu st.
+  destruct (read_precond_b fu st) eqn:Heq.
+  - left. unfold read_precond, read_precond_b, second_order_conflict in *.
+    apply andb_prop in Heq. destruct Heq as [Hbusy Hraw].
+    split. assumption.
+    apply negb_true_iff in Hraw.
+    intro Hcontra.
+    apply raw_hazard_iff in Hcontra.
+    rewrite Hcontra in Hraw. discriminate.
+  - right. unfold read_precond, read_precond_b, second_order_conflict in *.
+    intro Hcontra. destruct Hcontra as [Hbusy Hnoraw].
+    assert (Hraw: raw_hazard_b (sb_fu_status st fu) = false).
+    { destruct (raw_hazard_b (sb_fu_status st fu)) eqn:Hrb; [|reflexivity].
+      exfalso. apply Hnoraw. apply raw_hazard_iff. assumption. }
+    rewrite Hbusy in Heq. rewrite Hraw in Heq. simpl in Heq. discriminate.
+Qed.
+
 (** Read value from a register *)
 Definition read_reg (st : scoreboard_state) (r : reg_id) : nat :=
   match r with
@@ -1250,6 +1459,48 @@ Definition writeback_precond (fu : func_unit) (st : scoreboard_state) : Prop :=
   | None => False
   end.
 
+(** Boolean version of writeback_precond *)
+Definition writeback_precond_b (fu : func_unit) (st : scoreboard_state) : bool :=
+  let desc := sb_fu_status st fu in
+  andb (andb (fu_busy desc) (Nat.eqb (fu_remaining_cycles desc) 0))
+       (match fu_fi desc with
+        | Some dest => negb (reg_will_be_read (sb_fu_status st) dest)
+        | None => false
+        end).
+
+(** writeback_precond decidability *)
+Lemma writeback_precond_dec : forall fu st, {writeback_precond fu st} + {~writeback_precond fu st}.
+Proof.
+  intros fu st.
+  destruct (fu_busy (sb_fu_status st fu)) eqn:Hbusy.
+  - destruct (Nat.eqb (fu_remaining_cycles (sb_fu_status st fu)) 0) eqn:Hcyc.
+    + destruct (fu_fi (sb_fu_status st fu)) as [dest|] eqn:Hfi.
+      * destruct (reg_will_be_read (sb_fu_status st) dest) eqn:Hwar.
+        -- right. intro Hcontra.
+           unfold writeback_precond in Hcontra.
+           destruct Hcontra as [_ [_ Hnowar]].
+           rewrite Hfi in Hnowar.
+           apply Hnowar. unfold third_order_conflict, war_hazard. assumption.
+        -- left. unfold writeback_precond.
+           split. assumption.
+           split. apply Nat.eqb_eq. assumption.
+           rewrite Hfi. intro Hcontra.
+           unfold third_order_conflict, war_hazard in Hcontra.
+           rewrite Hcontra in Hwar. discriminate.
+      * right. intro Hcontra.
+        unfold writeback_precond in Hcontra.
+        destruct Hcontra as [_ [_ Hfalse]].
+        rewrite Hfi in Hfalse. exact Hfalse.
+    + right. intro Hcontra.
+      unfold writeback_precond in Hcontra.
+      destruct Hcontra as [_ [Hcyc0 _]].
+      apply Nat.eqb_eq in Hcyc0. rewrite Hcyc0 in Hcyc. discriminate.
+  - right. intro Hcontra.
+    unfold writeback_precond in Hcontra.
+    destruct Hcontra as [Hb _].
+    rewrite Hb in Hbusy. discriminate.
+Qed.
+
 (** Write value to a register *)
 Definition write_reg (st : scoreboard_state) (r : reg_id) (v : nat) : scoreboard_state :=
   match r with
@@ -1294,6 +1545,28 @@ Definition write_reg (st : scoreboard_state) (r : reg_id) (v : nat) : scoreboard
       (sb_mem st)
   end.
 
+(** Broadcast writeback: when FU completes, wake up waiting FUs by clearing matching Q-numbers *)
+Definition broadcast_writeback (fus : fu_status) (completed_fu : func_unit) : fu_status :=
+  fun fu' =>
+    let desc' := fus fu' in
+    if fu_busy desc' then
+      mk_fu_desc
+        (fu_busy desc')
+        (fu_op desc')
+        (fu_fi desc')
+        (fu_fj desc')
+        (fu_fk desc')
+        (if qnum_eq (fu_qj desc') (QFU completed_fu) then QNone else fu_qj desc')
+        (if qnum_eq (fu_qk desc') (QFU completed_fu) then QNone else fu_qk desc')
+        (if qnum_eq (fu_qj desc') (QFU completed_fu) then true else fu_rj desc')
+        (if qnum_eq (fu_qk desc') (QFU completed_fu) then true else fu_rk desc')
+        (fu_remaining_cycles desc')
+        (fu_operand1 desc')
+        (fu_operand2 desc')
+        (fu_result desc')
+        (fu_branch_target desc')
+    else desc'.
+
 (** Writeback transition: write computed result to register, free FU, clear register result status *)
 Definition writeback_transition (fu : func_unit) (st : scoreboard_state) : scoreboard_state :=
   let desc := sb_fu_status st fu in
@@ -1308,11 +1581,12 @@ Definition writeback_transition (fu : func_unit) (st : scoreboard_state) : score
                     | Some target, Some v => if Nat.eqb v 0 then sb_pc st_with_result else target
                     | _, _ => sb_pc st_with_result
                     end in
+      let broadcasted_fus := broadcast_writeback (sb_fu_status st_with_result) fu in
       increment_cycle (mk_sb_state
         (sb_xregs st_with_result)
         (sb_aregs st_with_result)
         (sb_bregs st_with_result)
-        (update_fu (sb_fu_status st_with_result) fu init_fu_desc)
+        (update_fu broadcasted_fus fu init_fu_desc)
         new_rrs
         (sb_instr_queue st_with_result)
         (sb_cycle_count st_with_result)
@@ -1412,6 +1686,7 @@ Inductive sb_step : scoreboard_state -> scoreboard_state -> Prop :=
       st' = read_transition fu st ->
       sb_step st st'
   | Step_Execute : forall st fu st',
+      fu_busy (sb_fu_status st fu) = true ->
       st' = execute_step fu st ->
       sb_step st st'
   | Step_Writeback : forall st fu st',
@@ -1611,7 +1886,7 @@ Proof. intro b. reflexivity. Qed.
 (** Helper lemma: reg_eq is reflexive *)
 Lemma reg_eq_refl : forall r, reg_eq r r = true.
 Proof.
-  intro r. unfold reg_eq. destruct r as [xr|ar|br]; destruct xr || destruct ar || destruct br; reflexivity.
+  intro r. apply reg_eq_spec. reflexivity.
 Qed.
 
 (** Helper lemma: if FU is busy with destination r, then reg_reserved returns true *)
@@ -2327,6 +2602,21 @@ Proof.
   - unfold b0_zero_inv in *. simpl. assumption.
 Qed.
 
+(** Broadcast preserves FU descriptor validity *)
+Lemma broadcast_preserves_fu_desc_valid : forall fus fu,
+  (forall fu', fu_desc_valid (fus fu')) ->
+  (forall fu', fu_desc_valid (broadcast_writeback fus fu fu')).
+Proof.
+  intros fus fu Hvalid fu'.
+  unfold broadcast_writeback.
+  destruct (fu_busy (fus fu')) eqn:Hbusy; [|apply Hvalid].
+  unfold fu_desc_valid. simpl.
+  destruct (Hvalid fu') as [Hqj [Hqk Hbranch]].
+  split. destruct (qnum_eq (fu_qj (fus fu')) (QFU fu)); [constructor | assumption].
+  split. destruct (qnum_eq (fu_qk (fus fu')) (QFU fu)); [constructor | assumption].
+  assumption.
+Qed.
+
 (** Writeback preserves FU descriptor validity *)
 Lemma writeback_preserves_fu_desc_valid : forall st fu,
   (forall fu', fu_desc_valid (sb_fu_status st fu')) ->
@@ -2337,14 +2627,29 @@ Proof.
   destruct (fu_fi (sb_fu_status st fu)) as [dest|] eqn:Hfi; try apply Hvalid.
   destruct (fu_result (sb_fu_status st fu)) as [v|] eqn:Hres.
   - unfold write_reg. destruct dest as [xr|ar|br]; simpl.
-    + apply update_fu_preserves_validity; try apply Hvalid;
-      unfold fu_desc_valid, init_fu_desc; simpl; split; [constructor | split; [constructor | intros target H; discriminate]].
-    + apply update_fu_preserves_validity; try apply Hvalid;
-      unfold fu_desc_valid, init_fu_desc; simpl; split; [constructor | split; [constructor | intros target H; discriminate]].
-    + apply update_fu_preserves_validity; try apply Hvalid;
-      unfold fu_desc_valid, init_fu_desc; simpl; split; [constructor | split; [constructor | intros target H; discriminate]].
-  - simpl. apply update_fu_preserves_validity; try apply Hvalid;
-    unfold fu_desc_valid, init_fu_desc; simpl; split; [constructor | split; [constructor | intros target H; discriminate]].
+    + apply update_fu_preserves_validity.
+      * apply broadcast_preserves_fu_desc_valid. assumption.
+      * unfold fu_desc_valid, init_fu_desc; simpl; split; [constructor | split; [constructor | intros target H; discriminate]].
+    + apply update_fu_preserves_validity.
+      * apply broadcast_preserves_fu_desc_valid. assumption.
+      * unfold fu_desc_valid, init_fu_desc; simpl; split; [constructor | split; [constructor | intros target H; discriminate]].
+    + apply update_fu_preserves_validity.
+      * apply broadcast_preserves_fu_desc_valid. assumption.
+      * unfold fu_desc_valid, init_fu_desc; simpl; split; [constructor | split; [constructor | intros target H; discriminate]].
+  - simpl. apply update_fu_preserves_validity.
+    + apply broadcast_preserves_fu_desc_valid. assumption.
+    + unfold fu_desc_valid, init_fu_desc; simpl; split; [constructor | split; [constructor | intros target H; discriminate]].
+Qed.
+
+(** Broadcast preserves busy consistency *)
+Lemma broadcast_preserves_busy_consistency : forall fus fu,
+  (forall fu', busy_consistency (fus fu')) ->
+  (forall fu', busy_consistency (broadcast_writeback fus fu fu')).
+Proof.
+  intros fus fu Hbusy fu'.
+  unfold broadcast_writeback.
+  destruct (fu_busy (fus fu')) eqn:Hfubusy; [|apply Hbusy].
+  unfold busy_consistency. simpl. intro H. discriminate.
 Qed.
 
 (** Writeback preserves busy consistency *)
@@ -2363,7 +2668,7 @@ Proof.
       | FU_LongAdd, FU_LongAdd | FU_FPAdd, FU_FPAdd | FU_FPMul1, FU_FPMul1
       | FU_FPMul2, FU_FPMul2 | FU_FPDiv, FU_FPDiv | FU_Incr1, FU_Incr1 | FU_Incr2, FU_Incr2 => true
       | _, _ => false
-    end) eqn:Heq; simpl; try apply Hbusy;
+    end) eqn:Heq; simpl; try (apply broadcast_preserves_busy_consistency; assumption);
     unfold busy_consistency, init_fu_desc; simpl; intros _; repeat split; reflexivity.
   - simpl. unfold busy_consistency, update_fu.
     destruct (match fu, fu' with
@@ -2371,8 +2676,22 @@ Proof.
       | FU_LongAdd, FU_LongAdd | FU_FPAdd, FU_FPAdd | FU_FPMul1, FU_FPMul1
       | FU_FPMul2, FU_FPMul2 | FU_FPDiv, FU_FPDiv | FU_Incr1, FU_Incr1 | FU_Incr2, FU_Incr2 => true
       | _, _ => false
-    end) eqn:Heq; simpl; try apply Hbusy;
+    end) eqn:Heq; simpl; try (apply broadcast_preserves_busy_consistency; assumption);
     unfold busy_consistency, init_fu_desc; simpl; intros _; repeat split; reflexivity.
+Qed.
+
+(** Broadcast preserves Rj correctness *)
+Lemma broadcast_preserves_rj_correct : forall fus fu,
+  (forall fu', rj_correctness (fus fu')) ->
+  (forall fu', rj_correctness (broadcast_writeback fus fu fu')).
+Proof.
+  intros fus fu Hrj fu'.
+  unfold broadcast_writeback.
+  destruct (fu_busy (fus fu')) eqn:Hbusy; [|apply Hrj].
+  unfold rj_correctness. simpl.
+  destruct (qnum_eq (fu_qj (fus fu')) (QFU fu)) eqn:Hqj.
+  - split; intros; reflexivity.
+  - apply Hrj.
 Qed.
 
 (** Writeback preserves Rj correctness *)
@@ -2391,7 +2710,7 @@ Proof.
       | FU_LongAdd, FU_LongAdd | FU_FPAdd, FU_FPAdd | FU_FPMul1, FU_FPMul1
       | FU_FPMul2, FU_FPMul2 | FU_FPDiv, FU_FPDiv | FU_Incr1, FU_Incr1 | FU_Incr2, FU_Incr2 => true
       | _, _ => false
-    end) eqn:Heq; simpl; try apply Hrj;
+    end) eqn:Heq; simpl; try (apply broadcast_preserves_rj_correct; assumption);
     unfold rj_correctness, init_fu_desc; simpl; split; intros; reflexivity.
   - simpl. unfold rj_correctness, update_fu.
     destruct (match fu, fu' with
@@ -2399,8 +2718,22 @@ Proof.
       | FU_LongAdd, FU_LongAdd | FU_FPAdd, FU_FPAdd | FU_FPMul1, FU_FPMul1
       | FU_FPMul2, FU_FPMul2 | FU_FPDiv, FU_FPDiv | FU_Incr1, FU_Incr1 | FU_Incr2, FU_Incr2 => true
       | _, _ => false
-    end) eqn:Heq; simpl; try apply Hrj;
+    end) eqn:Heq; simpl; try (apply broadcast_preserves_rj_correct; assumption);
     unfold rj_correctness, init_fu_desc; simpl; split; intros; reflexivity.
+Qed.
+
+(** Broadcast preserves Rk correctness *)
+Lemma broadcast_preserves_rk_correct : forall fus fu,
+  (forall fu', rk_correctness (fus fu')) ->
+  (forall fu', rk_correctness (broadcast_writeback fus fu fu')).
+Proof.
+  intros fus fu Hrk fu'.
+  unfold broadcast_writeback.
+  destruct (fu_busy (fus fu')) eqn:Hbusy; [|apply Hrk].
+  unfold rk_correctness. simpl.
+  destruct (qnum_eq (fu_qk (fus fu')) (QFU fu)) eqn:Hqk.
+  - split; intros; reflexivity.
+  - apply Hrk.
 Qed.
 
 (** Writeback preserves Rk correctness *)
@@ -2419,7 +2752,7 @@ Proof.
       | FU_LongAdd, FU_LongAdd | FU_FPAdd, FU_FPAdd | FU_FPMul1, FU_FPMul1
       | FU_FPMul2, FU_FPMul2 | FU_FPDiv, FU_FPDiv | FU_Incr1, FU_Incr1 | FU_Incr2, FU_Incr2 => true
       | _, _ => false
-    end) eqn:Heq; simpl; try apply Hrk;
+    end) eqn:Heq; simpl; try (apply broadcast_preserves_rk_correct; assumption);
     unfold rk_correctness, init_fu_desc; simpl; split; intros; reflexivity.
   - simpl. unfold rk_correctness, update_fu.
     destruct (match fu, fu' with
@@ -2427,8 +2760,20 @@ Proof.
       | FU_LongAdd, FU_LongAdd | FU_FPAdd, FU_FPAdd | FU_FPMul1, FU_FPMul1
       | FU_FPMul2, FU_FPMul2 | FU_FPDiv, FU_FPDiv | FU_Incr1, FU_Incr1 | FU_Incr2, FU_Incr2 => true
       | _, _ => false
-    end) eqn:Heq; simpl; try apply Hrk;
+    end) eqn:Heq; simpl; try (apply broadcast_preserves_rk_correct; assumption);
     unfold rk_correctness, init_fu_desc; simpl; split; intros; reflexivity.
+Qed.
+
+(** Broadcast preserves cycles bounded *)
+Lemma broadcast_preserves_cycles_bounded : forall fus fu,
+  (forall fu', cycles_bounded (fus fu')) ->
+  (forall fu', cycles_bounded (broadcast_writeback fus fu fu')).
+Proof.
+  intros fus fu Hcycles fu'.
+  unfold broadcast_writeback.
+  destruct (fu_busy (fus fu')) eqn:Hbusy; [|apply Hcycles].
+  unfold cycles_bounded. simpl. intro H. specialize (Hcycles fu').
+  unfold cycles_bounded in Hcycles. apply Hcycles. assumption.
 Qed.
 
 (** Writeback preserves cycles bounded *)
@@ -2447,7 +2792,7 @@ Proof.
       | FU_LongAdd, FU_LongAdd | FU_FPAdd, FU_FPAdd | FU_FPMul1, FU_FPMul1
       | FU_FPMul2, FU_FPMul2 | FU_FPDiv, FU_FPDiv | FU_Incr1, FU_Incr1 | FU_Incr2, FU_Incr2 => true
       | _, _ => false
-    end) eqn:Heq; simpl; try apply Hcycles;
+    end) eqn:Heq; simpl; try (apply broadcast_preserves_cycles_bounded; assumption);
     unfold cycles_bounded, init_fu_desc; simpl; intros H; discriminate.
   - simpl. unfold update_fu.
     destruct (match fu, fu' with
@@ -2455,7 +2800,7 @@ Proof.
       | FU_LongAdd, FU_LongAdd | FU_FPAdd, FU_FPAdd | FU_FPMul1, FU_FPMul1
       | FU_FPMul2, FU_FPMul2 | FU_FPDiv, FU_FPDiv | FU_Incr1, FU_Incr1 | FU_Incr2, FU_Incr2 => true
       | _, _ => false
-    end) eqn:Heq; simpl; try apply Hcycles;
+    end) eqn:Heq; simpl; try (apply broadcast_preserves_cycles_bounded; assumption);
     unfold cycles_bounded, init_fu_desc; simpl; intros H; discriminate.
 Qed.
 
@@ -2580,6 +2925,40 @@ Proof.
         -- assumption.
 Qed.
 
+(** Broadcast preserves fu_fi for the completing FU *)
+Lemma broadcast_preserves_fi : forall fus fu,
+  fu_fi (broadcast_writeback fus fu fu) = fu_fi (fus fu).
+Proof.
+  intros. unfold broadcast_writeback.
+  destruct (fu_busy (fus fu)) eqn:H; reflexivity.
+Qed.
+
+(** Broadcast preserves fu_busy for the completing FU *)
+Lemma broadcast_preserves_busy_self : forall fus fu,
+  fu_busy (broadcast_writeback fus fu fu) = fu_busy (fus fu).
+Proof.
+  intros. unfold broadcast_writeback. simpl.
+  destruct (fu_busy (fus fu)) eqn:H.
+  - simpl. reflexivity.
+  - simpl. rewrite H. reflexivity.
+Qed.
+
+(** Broadcast preserves register result consistency *)
+Lemma broadcast_preserves_reg_result_consistency : forall fus rrs fu,
+  reg_result_consistency fus rrs ->
+  reg_result_consistency (broadcast_writeback fus fu) rrs.
+Proof.
+  intros fus rrs fu Hreg fu'.
+  specialize (Hreg fu').
+  unfold broadcast_writeback.
+  destruct (fu_busy (fus fu')) eqn:Hbusy.
+  - exact Hreg.
+  - destruct (fu_fi (fus fu')) as [[xr|ar|br]|] eqn:Hfi; auto.
+    + intro H. rewrite Hbusy in H. discriminate.
+    + intro H. rewrite Hbusy in H. discriminate.
+    + intro H. rewrite Hbusy in H. discriminate.
+Qed.
+
 (** Writeback preserves register result consistency *)
 Lemma writeback_preserves_reg_result_consistency : forall st fu,
   writeback_precond fu st ->
@@ -2595,8 +2974,14 @@ Proof.
   - destruct (fu_result (sb_fu_status st fu)) as [v|] eqn:Hres.
     + rewrite write_reg_preserves_fu_status.
       rewrite write_reg_preserves_reg_result.
-      apply reset_fu_preserves_reg_result_consistency; assumption.
-    + apply reset_fu_preserves_reg_result_consistency; assumption.
+      apply reset_fu_preserves_reg_result_consistency.
+      * apply broadcast_preserves_reg_result_consistency. assumption.
+      * rewrite broadcast_preserves_fi. assumption.
+      * rewrite broadcast_preserves_busy_self. assumption.
+    + apply reset_fu_preserves_reg_result_consistency.
+      * apply broadcast_preserves_reg_result_consistency. assumption.
+      * rewrite broadcast_preserves_fi. assumption.
+      * rewrite broadcast_preserves_busy_self. assumption.
   - exfalso. exact Hdest.
 Qed.
 
@@ -3133,9 +3518,79 @@ Definition progress_property : Prop :=
   forall st, scoreboard_invariant st -> has_work st ->
     exists st', sb_step st st'.
 
-(** Determinism: steps are deterministic given same state *)
+(** Determinism: steps are deterministic given same state and same transition type *)
 Definition deterministic_step : Prop :=
   forall st st1 st2, sb_step st st1 -> sb_step st st2 -> st1 = st2.
+
+(** Note: The scoreboard allows multiple concurrent steps (e.g., Execute on FU1
+    while Read on FU2), so full determinism doesn't hold. Instead, we prove
+    determinism conditioned on the same transition being chosen. *)
+
+(** Same-transition determinism for Issue *)
+Lemma issue_deterministic : forall st instr1 instr2 st1 st2,
+  st1 = issue_transition st instr1 ->
+  st2 = issue_transition st instr2 ->
+  instr1 = instr2 ->
+  st1 = st2.
+Proof.
+  intros st instr1 instr2 st1 st2 H1 H2 Heq.
+  subst. reflexivity.
+Qed.
+
+(** Same-FU determinism for Read *)
+Lemma read_deterministic : forall st fu st1 st2,
+  st1 = read_transition fu st ->
+  st2 = read_transition fu st ->
+  st1 = st2.
+Proof.
+  intros st fu st1 st2 H1 H2.
+  subst. reflexivity.
+Qed.
+
+(** Same-FU determinism for Execute *)
+Lemma execute_deterministic : forall st fu st1 st2,
+  st1 = execute_step fu st ->
+  st2 = execute_step fu st ->
+  st1 = st2.
+Proof.
+  intros st fu st1 st2 H1 H2.
+  subst. reflexivity.
+Qed.
+
+(** Same-FU determinism for Writeback *)
+Lemma writeback_deterministic : forall st fu st1 st2,
+  st1 = writeback_transition fu st ->
+  st2 = writeback_transition fu st ->
+  st1 = st2.
+Proof.
+  intros st fu st1 st2 H1 H2.
+  subst. reflexivity.
+Qed.
+
+(** Fetch determinism *)
+Lemma fetch_deterministic : forall st st1 st2,
+  st1 = fetch_and_enqueue st ->
+  st2 = fetch_and_enqueue st ->
+  st1 = st2.
+Proof.
+  intros st st1 st2 H1 H2.
+  subst. reflexivity.
+Qed.
+
+(** Dispatch determinism *)
+Lemma dispatch_deterministic : forall st st1 st2,
+  st1 = issue_from_queue st ->
+  st2 = issue_from_queue st ->
+  st1 = st2.
+Proof.
+  intros st st1 st2 H1 H2.
+  subst. reflexivity.
+Qed.
+
+(** Observation: sb_step is NOT fully deterministic because multiple
+    transitions can fire simultaneously (e.g., execute on different FUs).
+    This is inherent to the concurrent nature of the scoreboard.
+    Each individual transition type IS deterministic given its parameters. *)
 
 (** Safety: all reachable states satisfy the invariant *)
 Definition safety_property : Prop :=
@@ -3243,7 +3698,7 @@ Proof.
   - apply not_quiescent_exists_busy in Hnq.
     destruct Hnq as [fu Hbusy].
     exists (execute_step fu st).
-    apply (Step_Execute st fu). reflexivity.
+    apply (Step_Execute st fu). assumption. reflexivity.
 Qed.
 
 (** Helper: if fetch precondition holds, we can fetch *)
@@ -3346,9 +3801,24 @@ Proof.
   apply (imem_has_instr_enables_fetch st instr); assumption.
 Qed.
 
-(** Note: Full no_deadlock requires modeling instruction memory population,
-    which is external to the scoreboard mechanism. The property holds when
-    imem contains valid instructions at the current PC. *)
+(** Stronger no_deadlock using invariant's imem_valid *)
+Theorem no_deadlock_from_invariant : forall st,
+  scoreboard_invariant st ->
+  quiescent st ->
+  sb_instr_queue st = [] ->
+  length (sb_instr_queue st) < MAX_QUEUE_DEPTH ->
+  (exists instr, sb_imem st (sb_pc st) = Some instr) ->
+  exists st', sb_step st st'.
+Proof.
+  intros st Hinv Hquiet Hempty Hlen [instr Himem].
+  apply fetch_enables_step.
+  apply (imem_has_instr_enables_fetch st instr); assumption.
+Qed.
+
+(** Note: Full no_deadlock without assuming imem contains instruction at PC
+    requires either totality of imem (all addresses map to instructions) or
+    modeling a halt state. The current formulation correctly captures that
+    progress is possible when imem has an instruction at the current PC. *)
 
 (** Functional units eventually complete: any busy FU will eventually become idle *)
 Definition eventual_completion : Prop :=
@@ -3376,13 +3846,52 @@ Definition eventual_completion : Prop :=
     The remaining challenge is proving WAR hazards eventually resolve,
     which requires reasoning about the dynamic behavior of read operations. *)
 
+Require Import Coq.Arith.Wf_nat.
+
+Definition fu_measure (st : scoreboard_state) (fu : func_unit) : nat :=
+  if fu_busy (sb_fu_status st fu)
+  then S (fu_remaining_cycles (sb_fu_status st fu))
+  else 0.
+
+Definition total_fu_cycles (st : scoreboard_state) : nat :=
+  fu_measure st FU_Branch + fu_measure st FU_Boolean + fu_measure st FU_Shift +
+  fu_measure st FU_LongAdd + fu_measure st FU_FPAdd + fu_measure st FU_FPMul1 +
+  fu_measure st FU_FPMul2 + fu_measure st FU_FPDiv + fu_measure st FU_Incr1 + fu_measure st FU_Incr2.
+
+Lemma execute_decreases_measure_for_fu : forall st fu,
+  fu_busy (sb_fu_status st fu) = true ->
+  fu_remaining_cycles (sb_fu_status st fu) > 0 ->
+  fu_measure (execute_step fu st) fu < fu_measure st fu.
+Proof.
+  intros st fu Hbusy Hcyc.
+  unfold fu_measure.
+  assert (Hdec := execute_decreases_cycles st fu Hbusy Hcyc).
+  assert (Hpres := execute_preserves_busy st fu Hbusy Hcyc).
+  rewrite Hpres. rewrite Hbusy. lia.
+Qed.
+
+Lemma execute_preserves_other_fu_measure : forall st fu fu',
+  fu <> fu' ->
+  fu_measure (execute_step fu st) fu' = fu_measure st fu'.
+Proof.
+  intros st fu fu' Hneq.
+  unfold fu_measure, execute_step.
+  destruct (fu_busy (sb_fu_status st fu)) eqn:Hb; [|reflexivity].
+  destruct (fu_remaining_cycles (sb_fu_status st fu) =? 0) eqn:Hc; [reflexivity|].
+  unfold increment_cycle, update_fu. simpl.
+  destruct (match fu, fu' with FU_Branch,FU_Branch|FU_Boolean,FU_Boolean|FU_Shift,FU_Shift
+           |FU_LongAdd,FU_LongAdd|FU_FPAdd,FU_FPAdd|FU_FPMul1,FU_FPMul1|FU_FPMul2,FU_FPMul2
+           |FU_FPDiv,FU_FPDiv|FU_Incr1,FU_Incr1|FU_Incr2,FU_Incr2 => true |_,_ => false end) eqn:Heq;
+  [exfalso; apply Hneq; destruct fu, fu'; try reflexivity; discriminate Heq|reflexivity].
+Qed.
+
 (** Helper: execute step can be taken for busy FU *)
 Lemma busy_fu_enables_execute_step : forall st fu,
   fu_busy (sb_fu_status st fu) = true ->
   sb_step st (execute_step fu st).
 Proof.
   intros st fu Hbusy.
-  apply (Step_Execute st fu). reflexivity.
+  apply (Step_Execute st fu). assumption. reflexivity.
 Qed.
 
 (** Helper: single execute step relates states *)
